replace use of Metalib atom with emtst atom to be compatible with Env.v

theories/Nom_SyntaxBST.v
@@ -5,23 +5,129 @@ Unset Strict Implicit.
 Unset Printing Implicit Defensive.
 Require Import Equations.Equations.
 From SendRec Require  Nom_Swap_fs.
-Require Import Metalib.Metatheory.
 Require Import Coq.ssr.ssreflect.
 Require Import Lia.
 Require Import PP.Ppsimplmathcomp.
 Require Import Equations.Equations.
+Require Import SendRec.Atom.
 
-Definition mem := AtomSetImpl.mem.
+Inductive sort : Set :=
+  | boole : sort (* boolean expression *)
+  | end_points : tp -> tp -> sort
+with tp : Set :=
+  | input : sort -> tp -> tp
+  | output : sort -> tp -> tp
+  | ch_input : tp -> tp -> tp
+  | ch_output : tp -> tp -> tp
+  | offer_branch : tp -> tp -> tp
+  | take_branch : tp -> tp -> tp
+  | ended : tp
+  | bot : tp
+.
+
+Scheme tp_sort := Induction for tp Sort Prop
+  with sort_tp := Induction for sort Sort Prop. (* Minimality *)
+Combined Scheme tp_sort_mutind from tp_sort, sort_tp.
+
+Fixpoint dual (T : tp) : tp :=
+  match T with
+  | input s T => output s (dual T)
+  | output s T => input s (dual T)
+  | ch_input T T' => ch_output T (dual T')
+  | ch_output T T' => ch_input T (dual T')
+  | offer_branch T T' => take_branch (dual T) (dual T')
+  | take_branch T T' => offer_branch (dual T) (dual T')
+  | ended => ended
+  | bot => bot
+  end
+.
+
+Lemma dual_is_dual t : dual (dual t) = t.
+  elim t=>// ; rewrite/dual ; move=>//; rewrite-/dual ;
+    do ? (move=> s t0 =>->) ;
+    do ? (move=> t0 R' t1 =>->) ;
+    rewrite ?R' ;
+   easy.
+Qed.
+
+Lemma double_dual t: t = dual(dual t).
+Proof.
+  elim t=>//; rewrite/dual=>//; rewrite-/dual ; congruence.
+Qed.
+
+Fixpoint eq_tp (T T': tp) : bool :=
+  match T, T' with
+  | input s T, input s' T' => eq_sort s s' && eq_tp T T'
+  | output s T, output s' T' => eq_sort s s' && eq_tp T T'
+  | ch_input T1 T2, ch_input T1' T2' => eq_tp T1 T1' && eq_tp T2 T2'
+  | ch_output T1 T2, ch_output T1' T2' => eq_tp T1 T1' && eq_tp T2 T2'
+
+  | offer_branch T1 T2, offer_branch T1' T2' => eq_tp T1 T1' && eq_tp T2 T2'
+  | take_branch T1 T2, take_branch T1' T2' => eq_tp T1 T1' && eq_tp T2 T2'
+  | ended, ended => true
+  | bot, bot => true
+  | _, _ => false
+  end
+with eq_sort (s s' : sort) : bool :=
+  match s, s' with
+  | boole, boole => true
+  | end_points T1 T2, end_points T1' T2' => eq_tp T1 T1' && eq_tp T2 T2'
+  | _, _ => false
+  end.
+
+Lemma eq_imp_eq : (forall x y, eq_tp x y -> x = y) /\ forall s s', eq_sort s s' -> s = s'.
+Proof.
+  apply tp_sort_mutind ; intros; try destruct y  ; try destruct s'; try easy ;
+  inversion H1 ; apply Bool.andb_true_iff in H3 ; destruct H3 ;
+  try(move:H3 ; move/H0=>H3 ; move:H2 ; move/H=>H4 ; by rewrite H3 H4).
+Qed.
+
+Lemma eq_tp_refl x : eq_tp x x.
+Proof.
+  by elim x using tp_sort with (P:=fun x=>eq_tp x x) (P0:= fun s=>eq_sort s s)=>//;
+     move=>s H t H0; simpl; rewrite H H0.
+Qed.
+
+Lemma eq_sort_refl s : eq_sort s s.
+Proof.
+  by elim s using sort_tp with (P:=fun x=> eq_tp x x)=>//;
+     move=>x H t H0; simpl; rewrite H H0.
+Qed.
+
+Lemma eq_tpP : Equality.axiom eq_tp.
+Proof.
+  move=>x y.
+  apply: (iffP idP)=>[|<-].
+  apply eq_imp_eq.
+  apply eq_tp_refl.
+Qed.
+
+Lemma eq_sortP : Equality.axiom eq_sort.
+Proof.
+  move=>x y.
+  apply: (iffP idP)=>[|<-].
+  apply eq_imp_eq.
+  apply eq_sort_refl.
+Qed.
+
+Canonical tp_eqMixin := EqMixin eq_tpP.
+Canonical tp_eqType := Eval hnf in EqType tp tp_eqMixin.
+
+Canonical sort_eqMixin := EqMixin eq_sortP.
+Canonical sort_eqType := Eval hnf in EqType sort sort_eqMixin.
+
 Inductive exp : Set :=
   | tt
   | ff
   | var : atom -> exp
 .
+
+Definition eq_atom := Atom.eq_atom.
 Definition exp_eqb e0 e1 : bool :=
 match (e0,e1) with
 | (tt,tt) => true
-| (ff,ff) => false 
-| (var nm0,var nm1) => eqb nm0 nm1
+| (ff,ff) => true
+| (var nm0,var nm1) => eq_atom nm0 nm1
 | _ => false
 end.
 
@@ -47,35 +153,37 @@ Notation "p0 |||| p1" := (par p0 p1)(at level 81, left associativity) .
 
 Fixpoint proc_eqb p0 p1 := 
 match p0,p1 with
-| (send a0 e0 p0'),(send a1 e1 p1') => eqb a0 a1 && exp_eqb e0 e1 && proc_eqb p0' p1'
-| (receive a0 a0' p0'),(receive a1 a1' p1') => eqb a0 a1 && eqb a0' a1' && proc_eqb p0' p1'
-| (throw a0 a0' p0'),(throw a1 a1' p1') => eqb a0 a1 && eqb a0' a1' && proc_eqb p0' p1'
-| (catch a0 a0' p0'),(catch a1 a1' p1') => eqb a0 a1 && eqb a0' a1' && proc_eqb p0' p1'
+| (send a0 e0 p0'),(send a1 e1 p1') => eq_atom a0 a1 && exp_eqb e0 e1 && proc_eqb p0' p1'
+| (receive a0 a0' p0'),(receive a1 a1' p1') => eq_atom a0 a1 && eq_atom a0' a1' && proc_eqb p0' p1'
+| (throw a0 a0' p0'),(throw a1 a1' p1') => eq_atom a0 a1 && eq_atom a0' a1' && proc_eqb p0' p1'
+| (catch a0 a0' p0'),(catch a1 a1' p1') => eq_atom a0 a1 && eq_atom a0' a1' && proc_eqb p0' p1'
 | (par p0' p0''),(par p1' p1'') => proc_eqb p0' p1' && proc_eqb p0'' p1''
 | inact,inact => true
-| nu_ch nm0 p0', nu_ch nm1 p1' => eqb nm0 nm1 && proc_eqb p0' p1'
+| nu_ch nm0 p0', nu_ch nm1 p1' => eq_atom nm0 nm1 && proc_eqb p0' p1'
 | _,_ => false 
 end.
 
-Definition fv_exp (e : exp) : atoms  :=
+Definition fv_exp (e : exp) : seq atom  :=
   match e with
-    | tt => {}
-    | ff => {}
-    | var a =>  {{ a }}
+    | tt => [::]
+    | ff => [::]
+    | var a =>  [::a]
   end.
 
-Fixpoint fv (P : proc) : atoms :=
+Fixpoint fv (P : proc) : seq atom :=
   match P with
-  | send nm e P0 => {{ nm }} `union` (fv_exp e) `union` (fv P0)
-  | receive nm0 nm1 P0 => {{ nm0 }} `union` (remove nm1 (fv P0))
-  | throw nm0 nm1 P0 => {{ nm0 }} `union` {{ nm1 }} `union` (fv P0)
-  | catch nm0 nm1 P0 => {{ nm0 }} `union` (remove nm1 (fv P0))
-  | par P0 P1 => (fv P0) `union` (fv P1)
-  | inact => {}
-  | nu_ch nm P0 => remove nm (fv P0)
+  | send nm e P0 => [::nm] ++ (fv_exp e) ++ (fv P0)
+  | receive nm0 nm1 P0 => [::nm0] ++ (filter (predC1 nm1) (fv P0))
+  | throw nm0 nm1 P0 => [::nm0; nm1] ++ (fv P0) 
+  | catch nm0 nm1 P0 => [::nm0] ++ (filter (predC1 nm1) (fv P0))
+  | par P0 P1 => (fv P0) ++ (fv P1)
+  | inact => [::]
+  | nu_ch nm P0 => filter (predC1 nm) (fv P0)
 end.          
 
-Definition swap_aux := Nom_Swap_fs.swap_aux.
+Definition swap_aux (b c a : atom) := 
+  if (a == b) then c else if (a == c) then b else a.
+
           
 Fixpoint swap_exp (b c : atom) (e: exp) : exp :=
   match e with
@@ -93,21 +201,21 @@ Fixpoint swap (b c: atom) (P : proc) : proc :=
   | inact => inact
   | nu_ch nm P0 => nu_ch (swap_aux b c nm) (swap b c P0)
   end.
-
+Print mem. Locate mem. Check mem_seq.
 Definition binder_eq f (p0 p1 : (atom * proc)) : bool :=
 let (nm0,P0) := p0 in let (nm1,P1) := p1 in
-if eqb nm0 nm1 then f P0 P1
-                               else if AtomSetImpl.mem nm0 (fv P1) then false 
+if eq_atom nm0 nm1 then f P0 P1
+                               else if mem_seq (fv P1) nm0 then false 
                                else f P0 (swap nm0 nm1 P1).
 
 
 Fixpoint aeq (P0 P1 : proc) : bool :=
 let binder_eq := binder_eq aeq in
 match P0,P1 with
-| (send nm0 e0 P0'), (send nm1 e1 P1') => (eqb nm0 nm1) && (exp_eqb e0 e1) && (aeq P0' P1')
-| (receive nm0 nmb0 P0'), (receive nm1 nmb1 P1') => (eqb nm0 nm1) && (binder_eq (nmb0, P0') (nmb1, P1'))
-| (throw nm0 nm0' P0'), (throw nm1 nm1' P1') => (eqb nm0 nm1) && (eqb nm0' nm1') && (aeq P0' P1')
-| (catch nm0 nmb0 P0'), (receive nm1 nmb1 P1') => (eqb nm0 nm1) && (binder_eq (nmb0, P0') (nmb1, P1'))
+| (send nm0 e0 P0'), (send nm1 e1 P1') => (eq_atom nm0 nm1) && (exp_eqb e0 e1) && (aeq P0' P1')
+| (receive nm0 nmb0 P0'), (receive nm1 nmb1 P1') => (eq_atom nm0 nm1) && (binder_eq (nmb0, P0') (nmb1, P1'))
+| (throw nm0 nm0' P0'), (throw nm1 nm1' P1') => (eq_atom nm0 nm1) && (eq_atom nm0' nm1') && (aeq P0' P1')
+| (catch nm0 nmb0 P0'), (receive nm1 nmb1 P1') => (eq_atom nm0 nm1) && (binder_eq (nmb0, P0') (nmb1, P1'))
 | (nu_ch nm0 P0), (nu_ch nm1 P1) => binder_eq (nm0, P0) (nm1, P1)
 | _, _ => false
 end.
@@ -132,7 +240,7 @@ else match P, Q with
      | (par inact P'),_ => proc_eqb P' Q
      | (par (par P' P'') P'''),(par Q' (par Q'' Q''')) => proc_eqb P' Q' && proc_eqb P'' Q'' && proc_eqb P''' Q''' 
      | (par P' P''),(par Q' Q'') => proc_eqb P' Q'' && proc_eqb P'' Q'
-     | (par (nu_ch nm P') P''), (nu_ch nm' (par Q' Q'')) => eqb nm nm' && proc_eqb P' Q' && proc_eqb P'' Q'' && (negb (AtomSetImpl.mem nm (fv P''))) 
+     | (par (nu_ch nm P') P''), (nu_ch nm' (par Q' Q'')) => eq_atom nm nm' && proc_eqb P' Q' && proc_eqb P'' Q'' && (negb (mem_seq (fv P'') nm)) 
      | (nu_ch m inact), inact => true 
      | _, _ => false 
      end.
@@ -141,7 +249,7 @@ else match P, Q with
 
 Definition subst_exp (e : exp) (x : atom) (e_body : exp) : exp :=
   match e_body with
-  | var nm => if eq_dec nm x then e else var nm
+  | var nm => if eq_atom nm x then e else var nm
   | t => t
   end.
 
@@ -168,34 +276,31 @@ Obligation Tactic := move => *;do ? ((do ? rewrite swap_size); apply : leP; rewr
 
 Equations subst_proc_exp (e : exp) (x : atom) (P : proc) : proc by wf (proc_size P)  :=
 subst_proc_exp e x (send nm e0 P0) := send nm (subst_exp e x e0) (subst_proc_exp e x P0);
-subst_proc_exp e x (receive nm0 nm1 P0) := if eqb x nm1 then  (receive nm0 nm1 P0) 
-                                                        else let (z,_) := atom_fresh (fv P0 `union`fv_exp e) in
-                                                             receive nm0 z (subst_proc_exp e x (swap nm1 z P0));
+subst_proc_exp e x (receive nm0 nm1 P0) := if eq_atom x nm1 then  (receive nm0 nm1 P0) 
+                                                        else receive nm0 (fresh (fv P0 ++ fv_exp e)) (subst_proc_exp e x (swap nm1 (fresh (fv P0 ++ fv_exp e)) P0));
 subst_proc_exp e x (throw nm0 nm1 P0) := throw nm0 nm1 (subst_proc_exp e x P0);
 subst_proc_exp e x (catch nm0 nm1 P0) := catch nm0 nm1 (subst_proc_exp e x P0);
 subst_proc_exp e x (par P0 P1) := par (subst_proc_exp e x P0) ( subst_proc_exp e x P1);
 subst_proc_exp e x inact := inact;
-subst_proc_exp e x (nu_ch nm P0) := nu_ch nm (subst_proc_exp e x P0).
-
+ subst_proc_exp e x (nu_ch nm P0) := nu_ch nm (subst_proc_exp e x P0).
 
 
 Definition subst_nm (a x nm : atom) : atom :=
-if eqb x nm then a else nm.
+if eq_atom x nm then a else nm.
 
 
 Equations subst_proc_nm (a x: atom)  (P : proc) : proc by wf (proc_size P)  :=
 subst_proc_nm a x (send nm e P0) := send (subst_nm a x nm) e (subst_proc_nm a x P0);
 subst_proc_nm a x (receive nm0 nm1 P0) := receive (subst_nm a x nm0) nm1 (subst_proc_nm a x P0);
 subst_proc_nm a x (throw nm0 nm1 P0) := throw (subst_nm a x nm0) (subst_nm a x nm1) (subst_proc_nm a x P0);
-subst_proc_nm a x (catch nm0 nm1 P0) := if eqb x nm1 then catch (subst_nm a x nm0) nm1 P0 
-                                                      else let (z,_) := atom_fresh (add a (fv P0) ) in 
-                                                              catch (subst_nm a x nm0) z (subst_proc_nm a x (swap nm1 z P0));
+subst_proc_nm a x (catch nm0 nm1 P0) := if eq_atom x nm1 then catch (subst_nm a x nm0) nm1 P0 
+                                                         else catch (subst_nm a x nm0) (fresh ([:: a]++ (fv P0))) (subst_proc_nm a x (swap nm1 (fresh ([:: a]++ (fv P0))) P0));
 subst_proc_nm a x (par P0 P1) := par (subst_proc_nm a x P0) ( subst_proc_nm a x P1);
 subst_proc_nm a x inact := inact;
-subst_proc_nm a x (nu_ch nm P0) := if eqb x nm then nu_ch nm P0 
-                                                else let (z,_) := atom_fresh (add a (fv P0)) in 
-                                                     nu_ch z (subst_proc_nm a x (swap nm z P0)).
+subst_proc_nm a x (nu_ch nm P0) := if eq_atom x nm then nu_ch nm P0 
+                                                   else nu_ch (fresh ([:: a] ++  (fv P0))) (subst_proc_nm a x (swap nm (fresh ([:: a] ++  (fv P0))) P0)).
 
+Reserved Notation "P --> Q" (at level 70).
 Inductive red : proc -> proc -> Prop :=
 | r_com k e nm P Q:
     (par (send k e P) (receive k nm Q)) --> (par P (subst_proc_exp e nm Q))
@@ -215,6 +320,7 @@ Inductive red : proc -> proc -> Prop :=
 
 where "P --> Q" := (red P Q).
 
+(*
 Ltac atom_destruct :=
   repeat match goal with
          | [ |- context[Atom.eq_dec ?e ?e0] ] 
@@ -223,7 +329,7 @@ Ltac atom_destruct :=
                 => destruct (Atom.eq_dec e e0);try contradiction
          end.
 
-Ltac atom_unf := rewrite /eqb ; atom_destruct.
+Ltac atom_unf := rewrite /eqb ; atom_destruct.*)
 
 Definition k0 := fresh [::].
 Definition k1 := fresh [::k0].
@@ -231,10 +337,15 @@ Definition k1 := fresh [::k0].
 Lemma ex1 : (k0![tt];inact |||| k0? (k1) in inact) --> (inact |||| inact).
 Proof. eapply r_com. Qed. 
 
+Lemma eq_atom_refl : forall a, eq_atom a a. 
+Proof.
+move=>a. apply/Atom.eq_reflect. auto. 
+Qed.
+
 (*Building on the simple example, instead of P -> inact |||| inact, we now have inact |||| P -> inact.
   Congruence rules must be used on both initial and reduced process before applying r_com.  *)
 Lemma ex_cong_comp : (inact |||| (k0![tt]; inact |||| k0? (k1) in inact)) --> inact.
-Proof. apply : r_cong. 2: { apply : ex1. } rewrite /=. atom_unf. rewrite /=//. rewrite /=//. 
+Proof. apply : r_cong. 2: { apply : ex1. } do ? rewrite /= eq_atom_refl //. rewrite /= //. 
 Qed.
 
 (*The inductive definition is useful when processes are to be manipulated (eg. change P to inact |||| P),
@@ -244,27 +355,23 @@ Lemma congruent_iff : forall P Q, P === Q <-> congruent_fun P Q.
 Proof. Admitted.
 
 (*The counter example that breaks subject reduction*)
-Lemma counter_ex : forall k0 k1 k2 k3, ((throw k0 k1 inact) |||| (catch k0 k2 (k2? (k3) in (k1![tt]; inact)))) -->
+Lemma counter_ex : forall k0 k1 k2 k3, k1 != k3 -> k1 != k2 -> ((throw k0 k1 inact) |||| (catch k0 k2 (k2? (k3) in (k1![tt]; inact)))) -->
                                     (k1? (k3) in (k1![tt]; inact)).
 Proof.
-move => k0 k1 k2 k3. apply : r_cong. rewrite -congruent_iff. apply : c_refl. 2: { rewrite -congruent_iff. apply : c_inact. } apply : r_cong. rewrite -congruent_iff. apply c_refl. apply : r_pass. destruct_notin. rewrite /fv. 
+move => k0 k1 k2 k3 H H2. apply : r_cong. rewrite -congruent_iff. apply : c_refl. 2: { rewrite -congruent_iff. apply : c_inact. } apply : r_cong. rewrite -congruent_iff. apply c_refl. apply : r_pass. rewrite /=.  rewrite H. simpl. rewrite inE /=. rewrite /negb /=. rewrite unfold_in. rewrite /=. Search _ (_ ||  false). rewrite Bool.orb_false_r. inversion H2. Search _ ( _ = true -> _ = false). destruct (eqVneq k1 k2). move : H1. rewrite /=. move=>H3. inversion H3. rewrite /=. rewrite eq_refl. 
 (*
-We are stuck on the goal 
-k1
-  `notin` union (singleton k2)
-            (remove k3 (union (singleton k1) (union (fv_exp tt) empty)))
-Since k1 is in the set
+We are stuck
 *)
 Abort. 
 
-Lemma eqb_refl : forall k, eqb k k.
-Proof. move=>k. atom_unf. done. Qed.
 
 (*We replace k1 with k2 in the receiving process, that way it does not end up with both sides of the channel*)
-Lemma counter_ex_fixed : forall k0 k1 k2 k3, k1 `notin` (singleton k1) -> 
+Lemma counter_ex_fixed : forall k0 k1 k2 k3, k1!= k2  -> k2 != k3 ->
   ((throw k0 k1 inact) |||| (catch k0 k2 (k2? (k3) in (k2![tt]; inact)))) -->
                                     (k1? (k3) in (k1![tt]; inact)).
 Proof.
-move => k0 k1 k2 k3 H. apply : r_cong. rewrite -congruent_iff. apply : c_refl. 2: { rewrite -congruent_iff. apply : c_inact. } apply : r_cong. rewrite -congruent_iff. apply c_refl. apply : r_pass. solve_notin. (*metalib tactic*)
-simp subst_proc_nm. rewrite /=. rewrite /subst_nm. do ? rewrite eqb_refl. rewrite /=//. 
+move => k0 k1 k2 k3 H H2. apply : r_cong. rewrite -congruent_iff. apply : c_refl. 2: { rewrite -congruent_iff. apply : c_inact. } apply : r_cong. rewrite -congruent_iff. apply c_refl. apply : r_pass. rewrite /=. rewrite inE.  
+rewrite unfold_in. destruct (eqVneq k1 k2). move : H=> /=. auto. rewrite /=. rewrite H2. rewrite /=. rewrite Bool.orb_false_r. auto.
+simp subst_proc_nm. rewrite /=. rewrite /subst_nm. do ? rewrite eq_atom_refl. rewrite /=//. 
 Qed.
+
